WIP: adding framework of threaded backward simulation for the C-assembly correctness

concur/VCompBig.v
@@ -5,6 +5,7 @@ Require Export Events.
 Require Export LanguageInterface.
 Require Export Smallstep.
 
+Require Import Relations.
 Require Import Axioms.
 Require Import Coqlib.
 Require Import Integers.
@@ -117,28 +118,179 @@ Proof.
 Qed.
 
 
-(** ** Identity *)
-(*
-Program Instance world_unit : World unit :=
-  {|
-    w_state := unit;
-    w_lens := lens_id;
-    w_acci := fun _ _ => True;
-    w_acce := fun _ _ => True;
-  |}.
+(** ** Composing two backward simulations *)
 
-Program Definition cc_id {li}: callconv li li :=
-  {|
-    ccworld := unit;
-    ccworld_world := world_unit;
-    match_senv w := eq;
-    match_query w := eq;
-    match_reply w := eq;
-  |}.
+Section COMPOSE_BACKWARD_SIMULATIONS.
 
-Solve All Obligations with
-  cbn; intros; subst; auto.
+Context {li1 li2 li3} {cc12: callconv li1 li2} {cc23: callconv li2 li3}.
+Context {state1 state2 state3: Type}.
+Variable L1: lts li1 li1 state1.
+Variable L2: lts li2 li2 state2.
+Variable L3: lts li3 li3 state3.
+Context (se1 se2 se3: Genv.symtbl) (w12: ccworld cc12) (w23: ccworld cc23).
+Context index order match_states (S12: bsim_properties cc12 se1 se2 w12 L1 L2 index order match_states).
+Context index' order' match_states' (S23: bsim_properties cc23 se2 se3 w23 L2 L3 index' order' match_states').
+Hypothesis L3_single_events: single_events L3.
 
-Notation "1" := cc_id : gs_cc_scope.
-*)
+Let bb_index : Type := (index * index')%type.
 
+Definition bb_order : bb_index -> bb_index -> Prop := lex_ord (clos_trans _ order) order'.
+
+Inductive bb_match_states:  gworld (cc_compose cc12 cc23) -> bb_index -> state1 -> state3 -> Prop :=
+  | bb_match_later: forall i1 i2 s1 s3 s2x s2y wp12 wp23,
+      match_states wp12 i1 s1 s2x -> Star L2 s2x E0 s2y -> match_states' wp23 i2 s2y s3 ->
+      bb_match_states (wp12, wp23) (i1, i2) s1 s3.
+
+Lemma bb_match_at: forall i1 i2 s1 s3 s2 wp12 wp23,
+  match_states wp12 i1 s1 s2 -> match_states' wp23 i2 s2 s3 ->
+  bb_match_states (wp12, wp23) (i1, i2) s1 s3.
+Proof.
+  intros. econstructor; eauto. apply star_refl.
+Qed.
+
+Lemma bb_simulation_base:
+  forall s3 t s3', Step L3 s3 t s3' ->
+  forall i1 s1 i2 s2 gw12 gw23, match_states gw12 i1 s1 s2 -> match_states' gw23 i2 s2 s3 -> safe L1 s1 ->
+  exists i', exists s1',
+    (Plus L1 s1 t s1' \/ (Star L1 s1 t s1' /\ bb_order i' (i1, i2)))
+    /\ bb_match_states (gw12, gw23) i' s1' s3'.
+Proof.
+  intros.
+  exploit (bsim_simulation' S23); eauto. eapply bsim_safe; eauto.
+  intros [ [i2' [s2' [PLUS2 MATCH2]]] | [i2' [ORD2 [EQ MATCH2]]]].
+- (* 1 L2 makes one or several transitions *)
+  assert (EITHER: t = E0 \/ (length t = 1)%nat).
+  { exploit L3_single_events; eauto.
+    destruct t; auto. destruct t; auto. simpl. intros. extlia. }
+  destruct EITHER.
++ (* 1.1 these are silent transitions *)
+  subst t. exploit (bsim_E0_plus S12); eauto.
+  intros [ [i1' [s1' [PLUS1 MATCH1]]] | [i1' [ORD1 MATCH1]]].
+* (* 1.1.1 L1 makes one or several transitions *)
+  exists (i1', i2'); exists s1'; split. auto. eapply bb_match_at; eauto.
+* (* 1.1.2 L1 makes no transitions *)
+  exists (i1', i2'); exists s1; split.
+  right; split. apply star_refl. left; auto.
+  eapply bb_match_at; eauto.
++ (* 1.2 non-silent transitions *)
+  exploit @star_non_E0_split. apply plus_star; eauto. auto.
+  intros [s2x [s2y [P [Q R]]]].
+  exploit (bsim_E0_star S12). eexact P. eauto. auto. intros [i1' [s1x [X Y]]].
+  exploit (bsim_simulation' S12). eexact Q. eauto. eapply star_safe; eauto.
+  intros [[i1'' [s1y [U V]]] | [i1'' [U [V W]]]]; try (subst t; discriminate).
+  exists (i1'', i2'); exists s1y; split.
+  left. eapply star_plus_trans; eauto. eapply bb_match_later; eauto.
+- (* 2. L2 makes no transitions *)
+  subst. exists (i1, i2'); exists s1; split.
+  right; split. apply star_refl. right; auto.
+  eapply bb_match_at; eauto.
+Qed.
+
+Lemma bb_simulation:
+  forall s3 t s3', Step L3 s3 t s3' ->
+  forall i s1, bb_match_states i s1 s3 -> safe L1 s1 ->
+  exists i', exists s1',
+    (Plus L1 s1 t s1' \/ (Star L1 s1 t s1' /\ bb_order i' i))
+    /\ bb_match_states i' s1' s3'.
+Proof.
+  intros. inv H0.
+  exploit star_inv; eauto. intros [[EQ1 EQ2] | PLUS].
+- (* 1. match at *)
+  subst. eapply bb_simulation_base; eauto.
+- (* 2. match later *)
+  exploit (bsim_E0_plus S12); eauto.
+  intros [[i1' [s1' [A B]]] | [i1' [A B]]].
++ (* 2.1 one or several silent transitions *)
+  exploit bb_simulation_base. eauto. auto. eexact B. eauto.
+    eapply star_safe; eauto. eapply plus_star; eauto.
+  intros [i'' [s1'' [C D]]].
+  exists i''; exists s1''; split; auto.
+  left. eapply plus_star_trans; eauto.
+  destruct C as [P | [P Q]]. apply plus_star; eauto. eauto.
+  traceEq.
++ (* 2.2 no silent transition *)
+  exploit bb_simulation_base. eauto. auto. eexact B. eauto. auto.
+  intros [i'' [s1'' [C D]]].
+  exists i''; exists s1''; split; auto.
+  intuition. right; intuition.
+  inv H6. left. eapply t_trans; eauto. left; auto.
+Qed.
+
+Lemma compose_bsim_match_cont:
+  forall k1 k2 k3,
+  bsim_match_cont (rex match_states) k1 k2 ->
+  bsim_match_cont (rex match_states') k2 k3 ->
+  bsim_match_cont (rex bb_match_states) k1 k3.
+Proof.
+  intros k1 k2 k3 [Hexist Hmatch] [Hexist' Hmatch'].
+  split.
+  - intros s1 Hs1. edestruct Hexist as [s2 Hs2]; eauto.
+  - intros s1 s3 Hs1 Hs3.
+    edestruct Hexist as (s2 & Hs2); eauto.
+    edestruct Hmatch' as (s2' & Hs2' & i' & M2); eauto.
+    edestruct Hmatch as (s1' & Hs1' & i & M1); eauto.
+    exists s1'; intuition auto. exists (i, i'). eapply bb_match_at; eauto.
+Qed.
+
+End COMPOSE_BACKWARD_SIMULATIONS.
+
+Lemma compose_backward_simulations:
+  forall {liA1 liA2 liA3} {ccA12: callconv liA1 liA2} {ccA23: callconv liA2 liA3},
+  forall {liB1 liB2 liB3} {ccB12: callconv liB1 liB2} {ccB23: callconv liB2 liB3},
+  forall L1 L2 L3,
+    backward_simulation ccA12 ccB12 L1 L2 ->
+    backward_simulation ccA23 ccB23 L2 L3 ->
+    (forall se3, single_events (L3 se3)) ->
+    backward_simulation (ccA12 @ ccA23) (ccB12 @ ccB23) L1 L3.
+Proof.
+  intros until L3. intros [H12] [H23] H3.
+  set (ms := fun se1 se3 '(se2, w12, w23) =>
+               bb_match_states (L2 se2) (bsim_match_states H12 se1 se2 w12)
+                                        (bsim_match_states H23 se2 se3 w23)).
+  constructor.
+  apply Backward_simulation with (bb_order (bsim_order H12) (bsim_order H23)) ms.
+  - (* skel *)
+    etransitivity; eapply bsim_skel; eauto.
+  - (* LTS *)
+    intros se1 se3 [[se2 wB12] wB23] [Hse12 Hse23] Hse1. cbn. clear ms.
+    assert (Hse2: Genv.valid_for (skel L2) se2).
+    { erewrite <- bsim_skel by eauto. eapply match_senv_valid_for; eauto. }
+    destruct H12 as [index12 order12 ms12 Hsk12 Hlts12 Hwf12]; cbn.
+    destruct H23 as [index23 order23 ms23 Hsk23 Hlts23 Hwf23]; cbn.
+    specialize (Hlts12 se1 se2 wB12 Hse12 Hse1).
+    specialize (Hlts23 se2 se3 wB23 Hse23 Hse2).
+    split.
+    + (* valid queries *)
+      intros q1 q3 (q2 & Hq12 & Hq23).
+      etransitivity; eapply bsim_match_valid_query; eauto.
+    + (* initial states *)
+      intros q1 q3 (q2 & Hq12 & Hq23).
+      eauto using compose_bsim_match_cont, bsim_match_initial_states.
+    + (* match final states *)
+      intros i s1 s3 r MS SAFE FIN. inv MS.
+      edestruct (bsim_match_final_states Hlts23) as (s2' & r2 & A & B & Hr23); eauto.
+        eapply star_safe; eauto. eapply bsim_safe; eauto.
+      edestruct (bsim_E0_star Hlts12) as (i1' & s1' & C & D).
+        eapply star_trans. eexact H0. eexact A. auto. eauto. auto.
+      edestruct (bsim_match_final_states Hlts12) as (s1'' & r1 & P & Q & Hr12); eauto.
+        eapply star_safe; eauto.
+      exists s1'', r1; cbn; split; eauto. eapply star_trans; eauto.
+    + (* external states *)
+      intros i s1 s3 q3 MS SAFE Hq3. destruct MS.
+      edestruct (bsim_match_external Hlts23) as (w23 & s2' & q2 & Hs2' & Hq2 & Hq23 & Hse23' & Hk23); eauto.
+        eapply star_safe; eauto. eapply bsim_safe; eauto.
+      edestruct (bsim_E0_star Hlts12) as (i' & s1' & Hs1' & Hs12').
+        eapply star_trans. eexact H0. eexact Hs2'. auto. eauto. auto.
+      edestruct (bsim_match_external Hlts12) as (w12 & s1'' & q1 & Hs1'' & Hq1 & Hq12 & Hse12' & Hk12); eauto.
+        eapply star_safe; eauto.
+      exists (se2, w12, w23), s1'', q1. cbn. repeat apply conj; eauto using star_trans.
+      intros r1 r3 (r2 & Hr12 & Hr23).
+      eapply compose_bsim_match_cont; eauto.
+    + (* progress *)
+      intros i s1 s3 MS SAFE. inv MS.
+      eapply (bsim_progress Hlts23). eauto. eapply star_safe; eauto. eapply bsim_safe; eauto.
+    + (* simulation *)
+      eapply bb_simulation; eauto.
+  - (* well founded *)
+    unfold bb_order. auto using wf_lex_ord, wf_clos_trans, bsim_order_wf.
+Qed.
